\item
$\qquad
f(x)=9x^2+6x+8
$
\item
$\qquad
f(x)=-3x^2+5x+5
$
\item
$\qquad
f(x)=8x^2+4x+9
$
\item
$\qquad
f(x)=4x^2-8x-8
$
\item
$\qquad
f(x)=-9x^2+5x+9
$
\item
$\qquad
f(x)=7x^2-8x+5
$
\item
$\qquad
f(x)=-4x^2-2x-7
$
\item
$\qquad
f(x)=6x^2-9x+3
$
\item
$\qquad
f(x)=5x^2+5x+7
$
\item
$\qquad
f(x)=-6x^2+7x+5
$
\item
$\qquad
f(x)=-9x^2-6x-7
$
\item
$\qquad
f(x)=-2x^2+9x+8
$
\item
$\qquad
f(x)=9x^2+x+4
$
\item
$\qquad
f(x)=9x^2-6x-5
$
\item
$\qquad
f(x)=-8x^2-7x-3
$
\item
$\qquad
f(x)=-3x^2-3x-6
$
\item
$\qquad
f(x)=-8x^2-6x+8
$
\item
$\qquad
f(x)=-x^2-6x-4
$
\item
$\qquad
f(x)=4x^2+8x-1
$
\item
$\qquad
f(x)=-4x^2+4x+5
$
\item
$\qquad
f(x)=-7x^2-4x+4
$
\item
$\qquad
f(x)=-7x^2+2x-4
$
\item
$\qquad
f(x)=-2x^2-8x+7
$
\item
$\qquad
f(x)=-4x^2+6x+9
$
\item
$\qquad
f(x)=-8x^2+5x+3
$
\item
$\qquad
f(x)=-3x^2-3x-2
$
\item
$\qquad
f(x)=5x^2+x+6
$
\item
$\qquad
f(x)=8x^2-4x-7
$
\item
$\qquad
f(x)=-4x^2-5x-3
$
\item
$\qquad
f(x)=-9x^2-9x-4
$
