\item Elev id: 2i 01
\begin{enumerate}
\item 
$$
f(x)=-4\cdot x^7+2\cdot x^7+21
$$
\item 
$$
f(x)=-5\cdot x^2-3\cdot \sqrt{x}+6\cdot x^{\frac{1}{2}}
$$
\item 
$$
f(x)=-1\cdot x^7+3\cdot e^{2\cdot x}-75
$$
\item 
$$
f(x)=4\cdot e^{2\cdot x}+6\cdot x^{\frac{1}{2}}-1\cdot e^{-3\cdot x}+4
$$
\end{enumerate}
\item Elev id: 2i 02
\begin{enumerate}
\item 
$$
f(x)=5\cdot x^{\frac{1}{2}}+8\cdot x+x^{\frac{1}{2}}
$$
\item 
$$
f(x)=-6\cdot x^{-5}+4\cdot x^{\frac{1}{2}}+73
$$
\item 
$$
f(x)=-5\cdot x^{-5}+x+28
$$
\item 
$$
f(x)=8\cdot \frac{1}{x}+7\cdot e^{2\cdot x}-5\cdot x-52
$$
\end{enumerate}
\item Elev id: 2i 03
\begin{enumerate}
\item 
$$
f(x)=6\cdot x^{-5}-6\cdot x^{-5}-45
$$
\item 
$$
f(x)=8\cdot x+2\cdot x^{-1}-3\cdot x^2+73
$$
\item 
$$
f(x)=9\cdot x^{-5}+8\cdot e^{-3\cdot x}-1\cdot e^{-3\cdot x}
$$
\item 
$$
f(x)=3\cdot x^7+8\cdot x^2-8\cdot \ln(x)+33
$$
\end{enumerate}
\item Elev id: 2i 04
\begin{enumerate}
\item 
$$
f(x)=-9\cdot e^{-3\cdot x}-8\cdot x^{-5}
$$
\item 
$$
f(x)=-3\cdot e^x+6\cdot x^{-1}-75
$$
\item 
$$
f(x)=8\cdot \ln(x)-7\cdot e^x
$$
\item 
$$
f(x)=4\cdot e^x+4\cdot \ln(x)
$$
\end{enumerate}
\item Elev id: 2i 05
\begin{enumerate}
\item 
$$
f(x)=x^{-1}+3\cdot e^{-3\cdot x}-9\cdot \frac{1}{x}-24
$$
\item 
$$
f(x)=2\cdot x+2\cdot x^{\frac{1}{2}}+45
$$
\item 
$$
f(x)=8\cdot x^7-1\cdot x^{\frac{1}{2}}-48
$$
\item 
$$
f(x)=-4\cdot x^{\frac{1}{2}}+9\cdot x^7+2\cdot x
$$
\end{enumerate}
\item Elev id: 2i 06
\begin{enumerate}
\item 
$$
f(x)=-3\cdot x^{-5}+6\cdot x^7-32
$$
\item 
$$
f(x)=2\cdot \ln(x)+x^{-1}-21
$$
\item 
$$
f(x)=5\cdot x^{-1}+5\cdot x^{\frac{1}{2}}
$$
\item 
$$
f(x)=-8\cdot x^{\frac{1}{2}}+7\cdot e^{-3\cdot x}-14
$$
\end{enumerate}
\item Elev id: 2i 07
\begin{enumerate}
\item 
$$
f(x)=-3\cdot \ln(x)+7\cdot e^x+5
$$
\item 
$$
f(x)=9\cdot e^{2\cdot x}-2\cdot \sqrt{x}+8\cdot x
$$
\item 
$$
f(x)=-1\cdot \ln(x)+3\cdot e^x
$$
\item 
$$
f(x)=9\cdot e^{2\cdot x}+3\cdot \sqrt{x}-2\cdot \frac{1}{x}+6
$$
\end{enumerate}
\item Elev id: 2i 08
\begin{enumerate}
\item 
$$
f(x)=-6\cdot x^{-5}-1\cdot x^7-5\cdot x^{-5}+36
$$
\item 
$$
f(x)=3\cdot \ln(x)-1\cdot e^{-3\cdot x}+5
$$
\item 
$$
f(x)=\frac{1}{x}-4\cdot e^{-3\cdot x}-5\cdot x^{-5}+86
$$
\item 
$$
f(x)=-3\cdot \sqrt{x}-6\cdot x^2+58
$$
\end{enumerate}
\item Elev id: 2i 09
\begin{enumerate}
\item 
$$
f(x)=2\cdot x^{\frac{1}{2}}+9\cdot e^x
$$
\item 
$$
f(x)=-9\cdot x^{-5}+5\cdot e^x-67
$$
\item 
$$
f(x)=2\cdot \ln(x)-8\cdot e^{2\cdot x}-95
$$
\item 
$$
f(x)=-3\cdot x^{-1}-9\cdot \frac{1}{x}-33
$$
\end{enumerate}
\item Elev id: 2i 10
\begin{enumerate}
\item 
$$
f(x)=5\cdot x+5\cdot x+48
$$
\item 
$$
f(x)=8\cdot x^2-3\cdot \sqrt{x}-4\cdot x^{-5}
$$
\item 
$$
f(x)=x^{\frac{1}{2}}+7\cdot x^{-1}-18
$$
\item 
$$
f(x)=6\cdot e^{-3\cdot x}+9\cdot e^x
$$
\end{enumerate}
\item Elev id: 2i 11
\begin{enumerate}
\item 
$$
f(x)=2\cdot \frac{1}{x}-3\cdot e^x+5\cdot \frac{1}{x}-17
$$
\item 
$$
f(x)=9\cdot x^7-3\cdot e^x-58
$$
\item 
$$
f(x)=3\cdot x-8\cdot e^{2\cdot x}-92
$$
\item 
$$
f(x)=3\cdot \sqrt{x}-5\cdot x+e^x-34
$$
\end{enumerate}
\item Elev id: 2i 12
\begin{enumerate}
\item 
$$
f(x)=-2\cdot e^x-6\cdot e^{2\cdot x}+6\cdot x^2-2
$$
\item 
$$
f(x)=6\cdot x^7-4\cdot x^{\frac{1}{2}}-8\cdot \sqrt{x}
$$
\item 
$$
f(x)=-2\cdot e^{2\cdot x}+8\cdot x^{-5}+3\cdot x^2
$$
\item 
$$
f(x)=-6\cdot e^{2\cdot x}-7\cdot \sqrt{x}+e^{-3\cdot x}-12
$$
\end{enumerate}
\item Elev id: 2i 13
\begin{enumerate}
\item 
$$
f(x)=3\cdot x^7+3\cdot e^{2\cdot x}-3\cdot \sqrt{x}-17
$$
\item 
$$
f(x)=-2\cdot x+5\cdot e^{2\cdot x}-9
$$
\item 
$$
f(x)=\ln(x)-5\cdot x+7\cdot x^{-5}
$$
\item 
$$
f(x)=4\cdot \ln(x)-3\cdot e^{-3\cdot x}-7\cdot e^{2\cdot x}+38
$$
\end{enumerate}
\item Elev id: 2i 14
\begin{enumerate}
\item 
$$
f(x)=-2\cdot \frac{1}{x}-7\cdot x^2-7\cdot x-2
$$
\item 
$$
f(x)=7\cdot x^7-1\cdot \ln(x)+39
$$
\item 
$$
f(x)=-5\cdot \ln(x)+x^7-8\cdot x^{-5}
$$
\item 
$$
f(x)=4\cdot \ln(x)+9\cdot \frac{1}{x}+71
$$
\end{enumerate}
\item Elev id: 2i 15
\begin{enumerate}
\item 
$$
f(x)=\ln(x)-2\cdot \sqrt{x}+9\cdot e^{-3\cdot x}-33
$$
\item 
$$
f(x)=-3\cdot x^{\frac{1}{2}}+2\cdot \ln(x)+55
$$
\item 
$$
f(x)=4\cdot e^{-3\cdot x}+8\cdot x^7+6\cdot x^{-1}-11
$$
\item 
$$
f(x)=-6\cdot x^{\frac{1}{2}}+3\cdot x^{\frac{1}{2}}+8\cdot x-59
$$
\end{enumerate}
\item Elev id: 2i 16
\begin{enumerate}
\item 
$$
f(x)=9\cdot x-7\cdot e^{-3\cdot x}-67
$$
\item 
$$
f(x)=-5\cdot x-2\cdot x^7-3\cdot x^{-5}-66
$$
\item 
$$
f(x)=7\cdot x^2-9\cdot x^{-1}
$$
\item 
$$
f(x)=-9\cdot x^2+9\cdot \sqrt{x}-8\cdot \sqrt{x}
$$
\end{enumerate}
\item Elev id: 2i 17
\begin{enumerate}
\item 
$$
f(x)=\sqrt{x}-6\cdot \ln(x)
$$
\item 
$$
f(x)=4\cdot e^x+3\cdot x^{-1}-82
$$
\item 
$$
f(x)=7\cdot e^{2\cdot x}+8\cdot x^{-5}-4\cdot e^x-78
$$
\item 
$$
f(x)=7\cdot e^x+5\cdot x-97
$$
\end{enumerate}
\item Elev id: 2i 18
\begin{enumerate}
\item 
$$
f(x)=-1\cdot x^2+2\cdot x^7-2\cdot e^x+51
$$
\item 
$$
f(x)=-4\cdot x^2-8\cdot \sqrt{x}+7\cdot e^{-3\cdot x}
$$
\item 
$$
f(x)=4\cdot x^7+2\cdot x^{\frac{1}{2}}+x^7-33
$$
\item 
$$
f(x)=6\cdot \ln(x)-7\cdot \ln(x)-23
$$
\end{enumerate}
\item Elev id: 2i 19
\begin{enumerate}
\item 
$$
f(x)=3\cdot e^{-3\cdot x}-4\cdot x^{\frac{1}{2}}-7\cdot x^2+46
$$
\item 
$$
f(x)=-1\cdot e^{2\cdot x}+4\cdot \ln(x)-2\cdot x^{-1}
$$
\item 
$$
f(x)=5\cdot \frac{1}{x}-8\cdot e^x+6\cdot x^{-5}-80
$$
\item 
$$
f(x)=5\cdot e^{2\cdot x}-7\cdot x^7+5\cdot x^{-1}
$$
\end{enumerate}
\item Elev id: 2i 20
\begin{enumerate}
\item 
$$
f(x)=6\cdot x^7+5\cdot x+74
$$
\item 
$$
f(x)=-6\cdot e^x+6\cdot x^{\frac{1}{2}}-4\cdot e^x
$$
\item 
$$
f(x)=e^{2\cdot x}+8\cdot x^{-5}
$$
\item 
$$
f(x)=6\cdot e^x+x^{\frac{1}{2}}-1\cdot x^2
$$
\end{enumerate}
\item Elev id: 2i 21
\begin{enumerate}
\item 
$$
f(x)=5\cdot \ln(x)-2\cdot e^{-3\cdot x}-8\cdot e^{2\cdot x}+52
$$
\item 
$$
f(x)=-4\cdot x^{\frac{1}{2}}+5\cdot x-57
$$
\item 
$$
f(x)=3\cdot x^2+3\cdot x-6\cdot x^{-5}+91
$$
\item 
$$
f(x)=4\cdot x^2+x-44
$$
\end{enumerate}
\item Elev id: 2i 22
\begin{enumerate}
\item 
$$
f(x)=9\cdot x^7+8\cdot \ln(x)+71
$$
\item 
$$
f(x)=5\cdot e^{2\cdot x}+2\cdot e^{2\cdot x}-82
$$
\item 
$$
f(x)=-3\cdot e^{2\cdot x}+9\cdot \frac{1}{x}+7\cdot x^{-1}-14
$$
\item 
$$
f(x)=-6\cdot x^{-1}-7\cdot \sqrt{x}
$$
\end{enumerate}
\item Elev id: 2i 23
\begin{enumerate}
\item 
$$
f(x)=x^{-5}-7\cdot \sqrt{x}-96
$$
\item 
$$
f(x)=-8\cdot \ln(x)-8\cdot \ln(x)-3\cdot e^x+44
$$
\item 
$$
f(x)=9\cdot x^{-1}+5\cdot x^{\frac{1}{2}}+7\cdot x^7
$$
\item 
$$
f(x)=-6\cdot \frac{1}{x}+8\cdot e^{2\cdot x}+2\cdot e^{2\cdot x}-28
$$
\end{enumerate}
\item Elev id: 2i 24
\begin{enumerate}
\item 
$$
f(x)=2\cdot e^{2\cdot x}+5\cdot x^2+32
$$
\item 
$$
f(x)=-5\cdot \ln(x)-4\cdot x-75
$$
\item 
$$
f(x)=-8\cdot e^{-3\cdot x}-2\cdot \ln(x)
$$
\item 
$$
f(x)=9\cdot x^{\frac{1}{2}}+6\cdot x^7-7\cdot x^{-5}+15
$$
\end{enumerate}
\item Elev id: 2i 25
\begin{enumerate}
\item 
$$
f(x)=3\cdot x^2-5\cdot \frac{1}{x}-2\cdot e^x-87
$$
\item 
$$
f(x)=-4\cdot \ln(x)-9\cdot \ln(x)
$$
\item 
$$
f(x)=-3\cdot x^{-1}+4\cdot \frac{1}{x}-1\cdot x^{-5}-66
$$
\item 
$$
f(x)=e^{-3\cdot x}-8\cdot \ln(x)-3\cdot x^{\frac{1}{2}}+23
$$
\end{enumerate}
\item Elev id: 2i 26
\begin{enumerate}
\item 
$$
f(x)=6\cdot \frac{1}{x}-9\cdot x^{\frac{1}{2}}
$$
\item 
$$
f(x)=6\cdot \frac{1}{x}+3\cdot e^{-3\cdot x}-7\cdot x^2+84
$$
\item 
$$
f(x)=6\cdot e^{2\cdot x}-5\cdot \sqrt{x}-62
$$
\item 
$$
f(x)=-5\cdot \ln(x)+3\cdot e^{-3\cdot x}-5\cdot x^7+80
$$
\end{enumerate}
\item Elev id: 2i 27
\begin{enumerate}
\item 
$$
f(x)=6\cdot x+8\cdot x+24
$$
\item 
$$
f(x)=-4\cdot \sqrt{x}+8\cdot x^7+x^7
$$
\item 
$$
f(x)=-4\cdot e^{-3\cdot x}-1\cdot x^{-5}+9\cdot \ln(x)-99
$$
\item 
$$
f(x)=4\cdot \ln(x)+5\cdot x^7+8
$$
\end{enumerate}
\item Elev id: 2i 28
\begin{enumerate}
\item 
$$
f(x)=-5\cdot e^x-2\cdot \ln(x)
$$
\item 
$$
f(x)=-6\cdot \ln(x)-6\cdot x^2
$$
\item 
$$
f(x)=-6\cdot \ln(x)-6\cdot \sqrt{x}+7\cdot x^7
$$
\item 
$$
f(x)=-3\cdot x^2+9\cdot x^{-5}
$$
\end{enumerate}
